local roots: Continued proofs, added store_to_local_root and load_from_local_root

theories/c_interop/notation.v
@@ -5,11 +5,22 @@ From iris.prelude Require Import options.
 Definition CAMLlocal (n:string) (e : expr) : expr :=
   (let: n := malloc (#1) in
     (Var n <- (call: &"int2val" with (Val (#0))));;
-    (call: &"registerroot" with (Var n));; e).
+    (call: &"registerlocalroot" with (Var n));; e).
 
 Notation "'CAMLlocal:' x 'in' e2" := (CAMLlocal x%string e2%CE)
   (at level 200, x at level 1, e2 at level 200,
    format "'[' 'CAMLlocal:'  x   'in'  '/' e2 ']'") : c_expr_scope.
+
+Notation "'caml_init_local' '(' ')'" := (call: &"initlocalroot" with ( ))%CE
+  (at level 70, format "'caml_init_local' '(' ')'") : c_expr_scope.
+
+Notation "'CAMLreturn' '(' x ')'" :=
+  (let: "!Hret" := x%CE in
+  (call: &"unregisterlocalroot" with ( ));;
+  ("!Hret"))%CE.
+
+(* XXX maybe make this list-based? *)
+Definition CAMLunregister1 ek := (call: &"unregisterroot" with ( ek ) ;; free (ek%CE, #1))%CE.
 
 Notation "'Field' '(' x ',' y ')'" := (call: &"readfield" with (x%CE, y%CE))%CE
   (at level 70, x, y at level 69,
@@ -42,7 +53,3 @@ Notation "'caml_alloc' '(' len ',' tag ')'" := (call: &"alloc" with (tag%CE, len
 Notation "'caml_alloc_custom' '(' ')'" := (call: &"alloc_foreign" with ( ))%CE
   (at level 70,
   format "'caml_alloc_custom' '(' ')'") : c_expr_scope.
-(* XXX maybe make this list-based? *)
-Definition CAMLunregister1 ek := (call: &"unregisterroot" with ( ek ) ;; free (ek%CE, #1))%CE.
-Notation "'CAMLreturn:' x 'unregistering' '[' e1 , .. , en ']'" := (let: "!Hret" := x%CE in (Seq (CAMLunregister1 e1%CE) .. (Seq (CAMLunregister1 en%CE) "!Hret"%CE) ..))%CE.
-
