theories/interop/wp_prims/registerlocalroot.v
@@ -30,6 +30,68 @@ Proof using.
   SI_at_boundary. iNamed "HGC". SI_GC_agree.
 
   iApply wp_pre_cases_c_prim; [done..|].
-Admitted.
+  iPoseProof (ghost_var_agree with "GCrootsf Hfc") as "->".
+  destruct roots_fm as [| fm roots_fm ]; first by simpl.
+  rewrite map_app in H2. simpl in H2.
+  iAssert (⌜¬ l ∈ dom fm⌝)%I as "%Hdom".
+  { iIntros "%H". eapply elem_of_dom in H. destruct H as [k Hk].
+  iDestruct "GCrootspto" as "((GCrootsptof&GCrootsptol)&GCrootsptog)".
+  iPoseProof (big_sepM_lookup_acc with "GCrootsptof") as "((%ww&Hww&_)&_)".
+  1: apply Hk. iPoseProof (resources.mapsto_ne with "Hpto Hww") as "%Hne". congruence. }
+
+  iExists (λ '(e', σ'),
+    e' = WrSE (ExprO (OVal #0)) ∧
+    σ' = CState {|
+      χC := χC ρc;
+      ζC := ζC ρc;
+      θC := θC ρc;
+      rootsC := ({[l]} ∪ (dom fm)) :: (map dom roots_fm) ++ [dom roots_gm]
+   |} mem).
+  iSplit. { iPureIntro. econstructor; eauto. }
+  iIntros (w' ρc' mem' (? & ?)); simplify_eq.
+  iDestruct "GCrootsm" as "(GCrootsfm&GCrootsm)".
+  iDestruct "Hlr" as "(%fm'&(Hlr1&%Hlr2))".
+  iPoseProof (ghost_map_auth_agree with "Hlr1 GCrootsfm") as "->".
+  iMod (ghost_var_update_halves with "SIroots GCroots") as "(SIroots&GCroots)".
+
+  iCombine "GCrootsfm Hlr1" as "GCrootsfm".
+  iMod (ghost_map_insert l v with "GCrootsfm") as "(GCrootsfm&Hres)".
+  1: eapply not_elem_of_dom; intros Hc; eapply Hdom; done.
+  iDestruct "GCrootsfm" as "(GCrootsfm&Hlr1)".
+
+  iDestruct "GCrootspto" as "((GCrootsptof&GCrootsptol)&GCrootsptogg)".
+  iPoseProof (big_sepM_insert) as "(_&HR)".
+  1: eapply not_elem_of_dom; intros Hc; eapply Hdom; done.
+  iPoseProof ("HR" with "[Hpto GCrootsptof]") as "GCrootsptof".
+  1: iFrame "GCrootsptof"; iExists w; iFrame; done.
+  iClear "HR".
+
+  iMod (ghost_var_update_halves with "GCrootsf Hfc") as "(GCrootsf&Hfc)".
+
+  iAssert (([∗ list] y1;y2 ∈ (f::fc);(<[l:=v]>fm::roots_fm), ghost_map_auth y1 (1/2) y2))%I
+  with "[GCrootsm GCrootsfm]" as "GCrootsm".
+  { simpl. iSplitL "GCrootsfm"; done. }
+
+  iAssert (local_roots f ({[l]} ∪ r)) with "[Hlr1]" as "Hlr".
+  { unfold local_roots. iExists (<[l:=v]> fm). iFrame. iPureIntro.
+    rewrite dom_insert_L. by rewrite Hlr2. }
+
+  do 3 iModIntro. iFrame. iSplitL "SIinit". { iExists false. iFrame. }
+  iApply wp_outcome; first done.
+  iApply "Hcont". iFrame.
+  iApply "Cont". iFrame "Hres Hfc Hlr".
+  iExists _, _, _, _, (<[l:=v]> fm :: roots_fm), roots_gm, _. unfold named. iFrame.
+  iPureIntro; split_and!; eauto.
+  - rewrite map_app. simpl. f_equal. by rewrite dom_insert_L.
+  - apply Forall_app.
+    unfold roots_are_live in Hrootslive. rewrite Forall_app in Hrootslive.
+    destruct Hrootslive as [Hrootslivel Hrootsliveg].
+    split; last done.
+    apply Forall_cons_1 in Hrootslivel.
+    destruct Hrootslivel as [Hrootslivefm Hrootslivef].
+    econstructor; last done.
+    intros ℓ γ [[-> ->]|[Hne HH]]%lookup_insert_Some; last by eapply Hrootslivefm.
+    inv_repr_lval. by eapply elem_of_dom_2.
+Qed.
 
 End Laws.
